refactoring using Records and Sections

Diff/ChainModel.v
@@ -4,51 +4,38 @@ Require Import LanguageModel.
 Require Import Galois. 
 Require Import MyNotation.
 
-Module Type RelTrace (TSource TTarget : Trace).
+
+Record CompilationChain (Source Target : Language) := { 
   
-  Parameter rel: TSource.trace -> TTarget.trace -> Prop.
+   compile_whole : prg Source -> prg Target;
+   compile_par   : par Source -> par Target;
+   compile_ctx   : ctx Source -> ctx Target
 
-  Module SProp := Properties TSource.
-  Module TProp := Properties TTarget. 
+  }. 
+
+
+(* Section RelTrace. *)
+
+(*   Variable Σ__S Σ__T States__S States__T : Set. *)
+(*   Variable E__S : Events Σ__S. *)
+(*   Variable E__T : Events Σ__T. *)
+(*   Variable S__S : EndState States__S. *)
+(*   Variable S__T : EndState States__T. *)
+
+(*   Local Definition trace__S := trace Σ__S States__S.  *)
+(*   Local Definition trace__T := trace Σ__T States__T.   *)
   
-  Definition prop__S := SProp.prop.
-  Definition prop__T := TProp.prop. 
+(*   Parameter rel: trace__S -> trace__T -> Prop. *)
 
-  Definition adjunction :=  induced_connection rel.  
+(*   Local Definition prop__S := prop Σ__S States__S. *)
+(*   Local Definition prop__T := prop Σ__T States__T. *)
   
-  Definition τ' : prop__S -> prop__T := α adjunction.   
-  Definition σ' : prop__T -> prop__S := γ adjunction.  
-
-  Definition rel_adjunction_law : Adjunction_law τ' σ' := adjunction_law adjunction. 
-      
-End RelTrace.
-
-Module Type CompilationChain (Source Target : Language). 
+(*   Definition adjunction :=  induced_connection rel.   *)
   
-  Parameter compile_whole : Source.prg -> Target.prg.
-  Parameter compile_par   : Source.par -> Target.par.
-  Parameter compile_ctx   : Source.ctx -> Target.ctx.
-  
-End CompilationChain. 
+(*   Definition τ' : prop__S -> prop__T := α adjunction.    *)
+(*   Definition σ' : prop__T -> prop__S := γ adjunction.   *)
 
-Module Type TCtilde_Chain (TSource TTarget : Trace)
-                          (R : RelTrace TSource TTarget)
-                          (Source Target : Language)  <:
-                          (CompilationChain Source Target).
+(*   Definition rel_adjunction_law : Adjunction_law τ' σ' := adjunction_law adjunction.  *)
 
-  Module Sat__S := Sat TSource Source.
-  Module Sat__T := Sat TTarget Target.
+(* End RelTrace. *)
 
-  Definition sem__S := Sat__S.sem.
-  Definition sem__T := Sat__T.sem.
-
-  (*CA: probably there is a way to not to write again these compile_* *)
-  Parameter compile_whole : Source.prg -> Target.prg.
-  Parameter compile_par   : Source.par -> Target.par.
-  Parameter compile_ctx   : Source.ctx -> Target.ctx.
-
-  Notation "W ↓" := (compile_whole W) (at level 50).
-                   
-  Parameter correctness : forall W__S t__T, sem__T (W__S ↓) t__T -> exists t__S, R.rel t__S t__T.
-  
-End TCtilde_Chain.
