Diff/NonRobustDef.v
@@ -1,7 +1,6 @@
 From mathcomp Require Import all_ssreflect. 
 
 Set Implicit Arguments.
-Unset Strict Implicit.
 Unset Printing Implicit Defensive.
 
 Require Import ClassicalExtras.
@@ -17,58 +16,75 @@ Require Import ChainModel.
 
 Hypothesis prop_extensionality : forall A B : Prop, (A <-> B) -> A = B.
 
-Module Preservation (TSource TTarget : Trace)
-                         (Source Target : Language)
-                         (Compiler : CompilationChain Source Target).
+Section Preservation.
+
+  Variable Source Target: Language.
+  Variable compilation_chain : CompilationChain Source Target.
   
-  Definition trace__S := TSource.trace.
-  Definition trace__T := TTarget.trace.
+  Variable Σ__S Σ__T States__S States__T : Set.
+  Variable E__S : Events Σ__S.
+  Variable E__T : Events Σ__T.
+  Variable S__S : EndState States__S.
+  Variable S__T : EndState States__T.
 
-  Module SProp := Properties TSource.
-  Module TProp := Properties TTarget. 
+  Local Definition trace__S := trace Σ__S States__S. 
+  Local Definition trace__T := trace Σ__T States__T.  
+  Local Definition prop__S := prop Σ__S States__S.
+  Local Definition prop__T := prop Σ__T States__T.
+
+  Variable sem__S : prg Source -> trace__S -> Prop.
+  Variable non_empty_sem__S : forall W, exists s, sem__S W s.   
+
+  Variable sem__T : prg Target -> trace__T -> Prop.
+  Variable non_empty_sem__T : forall W, exists t, sem__T W t.   
   
-  Definition prop__S := SProp.prop.
-  Definition prop__T := TProp.prop.
+  Local Definition prg__S := prg Source.
+  Local Definition prg__T := prg Target.
 
-  Definition prg__S := Source.prg.
-  Definition prg__T := Target.prg.
-
-  Module Sat__S := Sat TSource Source.  
-  Module Sat__T := Sat TTarget Target.
-
-  Definition sat__S := Sat__S.sat.
-  Definition sat__T := Sat__T.sat.
-
-  Definition cmp := Compiler.compile_whole.
-
-  Notation "W ↓" := (cmp W) (at level 50). 
+  Local Definition sat__S := sat Source sem__S.
+  Local Definition sat__T := sat Target sem__T.
   
+  Local Definition cmp := compile_whole Source Target compilation_chain.
+
+  Local Notation "W ↓" := (cmp W) (at level 50).  
+
   (* parameters *)
   
-  Parameter σ : prop__T -> prop__S.
-  Parameter τ : prop__S -> prop__T.
+  Variable σ : prop__T -> prop__S.
+  Variable τ : prop__S -> prop__T.
 
   (* definitions *)
+  
 
   Definition σP (W : prg__S) (π__T : prop__T) :=
     sat__S W (σ π__T) -> sat__T (W ↓) π__T.
 
-  Definition σTP := forall W π__T, σP W π__T. 
+  Definition σTP := forall W π__T, σP W π__T.
+
+  Lemma contra_σTP :
+    σTP <-> (forall W π__T, (exists t, sem__T (W ↓) t /\ ~ (π__T t)) ->
+                    (exists s, sem__S W s /\ ~ (σ π__T) s)).
+  Proof. Admitted. (*TODO: see contra_σRTP in previous files *)
   
   Definition τP (W : prg__S) (π__S : prop__S) :=
     sat__S W π__S -> sat__T (W ↓) (τ π__S).
 
   Definition τTP := forall W π__S, τP W π__S.
 
+   Lemma contra_τTP :
+    τTP <-> (forall W π__S, (exists t, sem__T (W ↓) t /\ ~ (τ π__S) t) ->
+                    (exists s, sem__S W s /\ ~ π__S s)).
+  Proof. Admitted. (*TODO: see contra_τRTP in previous files *)
+
   Theorem G_σTP_iff_τTP :
     (Galois_fst τ σ) -> (Galois_snd τ σ) -> (σTP <-> τTP).
   Proof.
      move => G1 G2. split. 
      - move => Hσ P πs Hsat_src. apply: (Hσ P (τ πs)).
-       apply: Sat__S.sat_upper_closed. exact Hsat_src. by apply: G1. 
+       apply: sat_upper_closed. exact Hsat_src. by apply: G1. 
      - move => Hτ P πt Hrsat_tgt.
        have H : sat__T (P ↓) (τ (σ πt)) by apply: Hτ. 
-       apply: Sat__T.sat_upper_closed. exact H. by apply: G2.
+       apply: sat_upper_closed. exact H. by apply: G2.
   Qed.     
 
   Corollary Adj_σTP_iff_τTP :
